new bank theorem

src/bank.v
@@ -1,5 +1,10 @@
+(*! A simple demo of Iris and Coq following tchajed/iris-bank-demo and article
+https://plv.csail.mit.edu/blog/iris-intro.html *)
+
 From iris.base_logic Require Import lib.ghost_var.
 
+(* This code is written in HeapLang, a simple ML-like language shipped with
+Iris. *)
 From iris.heap_lang Require Import proofmode notation adequacy.
 From iris.heap_lang.lib Require Import lock spin_lock.
 
@@ -50,12 +55,14 @@ Definition demo_check_consistency: val :=
     Fork (transfer "bank" #5);;
     check_consistency "bank".
 
-(* Section heap.
+Section heap.
 
-Context `{!heapG Σ}.
+(* mostly standard boilerplate *)
+Context `{!heapGS Σ}.
 Context `{!lockG Σ}.
-Context `{!inG Σ (ghostR ZO}}.
-Let N := nroot.@"bank". *)
+Context `{!ghost_varG Σ Z}.
+Let N := nroot.@"bank".
+
 
 (*
 Lemma ghost_var_alloc a :
@@ -84,20 +91,131 @@ Proof.
     { apply excl_auth_update. }
     done.
 Qed.
+*)
 
+(** Verifying concurrent software generally require the use of _ghost_state_.
+variables that are introduced into the program only for the sake of the proof.
+In some systems (like Dafny or VeriFast), ghost variables actually show up in
+the source code for the program being verified. In Iris, we'll only see ghost
+variables in the proof.
 
-Definition account_inv γ bl_ref : iProp Σ :=
-    ∃ (bal: Z), bal_ref ↦ #bal ∗ own γ (◯E bal).
+We'll now start writing down the invariant for this proof, and this is where
+we'll reference the ghost variables. We do that with a proposition [ghost_var γ
+q v], which says that the ghost variable with name [gamma] has value [v], and we
+own a fraction [q] (≤1) of it. Ghost variables in Iris are always a combination
+of knowledge about the variable and ownership over it. The key idea is that to
+change a ghost variable we need to assemble all the pieces of it, adding up to
+a fraction of 1; this guarantees that no other thread is claiming ownership and
+makes it sound to change its value without invalidating over thread's proofs. *)
 
+(** account_inv is the lock invariant associated with each account. It exposes a
+ghost name [γ] used to tie the account balance to a ghost variable. In the lock
+invariant we'll claim half ownership, while the other half will be in a
+system-wide invariant; this lets us reference the variable's value from both
+places and also assert that the lock is needed to change this balance. *)
+Definition account_inv γ bal_ref : iProp Σ :=
+    ∃ (bal: Z), bal_ref ↦ #bal ∗ ghost_var γ (1/2) bal.
+
+(** an account is a pair of a lock and an account protected by the lock *)
 Definition is_account (acct: val) γ : iProp Σ :=
-  ∃ (bal_ref: loc) lk,
-    ⌜acct = (lk, #bal_ref)%V⌝ ∗
-    ∃ (γ1: gname), is_lock γ1 lk (account_inv γ bal_ref).
+    ∃ (bal_ref: loc) lk,
+        ⌜acct = (lk, #bal_ref)%V⌝ ∗
+        (* The important part of [is_lock] is the lock invariant, expressed as
+        an arbitrary Iris proposition [iProp Σ]. The idea of lock invariants is
+        that first we associate a lock invariant [P] with the lock (we're doing
+        that here). Then when we acquire the lock we get (resources satisfying)
+        [P], and when we release it we have to give back (resources satisfying)
+        [P]. Crucially during the critical section we have access to [P] and can
+        violate this proposition freely. *)
+        ∃ (γ1: gname), is_lock γ1 lk (account_inv γ bal_ref).
 
-Definition bank_inv (γ: gname ∗ gname) : iProp Σ :=
-∃ (bal1 bal2: Z),
-    own γ.1 (●E bal1) ∗
-    own γ.2 (●E bal2) ∗
-    ⌜(bal1 + bal2)%Z = 0⌝.
+(* Not sure how I could differentiate * and ∗ in the following *)
+(** bank_inv is the invariant (the usual one that holds at all intermediate
+points) that holds the authoritative fragments for the account balances and
+importantly states that they are always equal. Any thread can open the invariant
+to "read" the logical balances, but modifications must respect the constraint
+here.
 
- *)
+We need to say where th logical (ghost) account balances are stored so this
+definition also takes two ghost names.
+
+As mentioned above, we claim half ownership to reference the value of both ghost
+variables. This half is a bit different because it's in a regular invariant,
+so any thread can open this invariant to learn the logical balances sum to
+zero. *)
+Definition bank_inv (γ: gname * gname) : iProp Σ :=
+    ∃ (bal1 bal2: Z),
+        ghost_var γ.1 (1/2) bal1 ∗
+        ghost_var γ.2 (1/2) bal2 ∗
+        ⌜(bal1 + bal2)%Z = 0⌝.
+
+(** finally [is_bank] ties everything together, the accounts and invariant *)
+Definition is_bank (b: val): iProp Σ :=
+    ∃ (acct1 acct2:val) (γ: gname*gname),
+    ⌜b = (acct1, acct2)%V⌝ ∗
+    is_account acct1 γ.1 ∗
+    is_account acct2 γ.2 ∗
+    inv N (bank_inv γ).
+
+(* Imporantly [is_bank b] is _persistent_, which means we can share it among
+threads. We'l see this used in [wp_demo_check_consistency].
+
+This proofs goes through because the componenets of [is_bank] are persistent.
+These include the pure facts (it should be intuitive that these are persistent,
+since they don't talk about resources at all), the invariant (because [inv N P]
+is just knowledge of an invariant, which can and should be shared) and
+[is_lock yl lk p] (similarly, this is knowledge that there is a lock at lk and
+is shareable). *)
+Instance is_bank_Persistent b : Persistent (is_bank b).
+Proof. apply _. (* this proof is actually automatic *) Qed.
+
+(* [new_bank] is actually interesting because we have to create all the ghost
+state, lock invariants, and invariant, and of course when you create an
+invariant holding [P] you have to prove [P].
+
+These ghost operations correspond to [iMod] in these proofs, which use theorems
+with [|==>] and [==∗]. *)
+Theorem wp_new_bank :
+    (* This is a Hoare triple using Iris' program logic. *)
+    {{{ True }}}
+        new_bank #()
+        (* the [b,] part is a shorthand for [∃ b, ...] in the postcondition, and
+        [RET b] says the function returns b. *)
+    {{{ b, RET b; is_bank b }}}.
+Proof.
+    iIntros (Φ) "_ HΦ".
+    wp_rec. (* unfold new_bank and runs a step of reduction *)
+    wp_alloc a_ref as "Ha".
+    wp_alloc b_ref as "Hb".
+    (* The first interesting step of the proof is that we execute the ghost
+    variable change in [ghost_var_alloc] and at the same time destruct it with
+    [as (γ1) "(Hown1&Hγ1)"], using [γ1] for the ghost name and [Hown1] and
+    [Hγ1] for the two halves, respectively. *)
+    iMod (ghost_var_alloc 0) as (γ1) "(Hown1&Hy1)".
+    wp_pures.
+    (* Now we can initialize the lock invariant for the first acount, which
+    will own the auth ["Hγ1"] created above. *)
+    wp_apply (newlock_spec (account_inv γ1 a_ref) with "[Ha Hγ1]").
+    { iExists _; iFrame. }
+    iIntros (lk_a γlk1) "Hlk1".
+    iMod (ghost_var_alloc 0) as (γ2) "(Hown2&Hy2)".
+    wp_pures.
+    wp_apply (newlock_spec (account_inv γ2 b_ref) with "[Hb Hγ2]").
+    { iExists _; iFrame. }
+    iIntros (lk_b γlk2) "Hlk2".
+    wp_pures.
+    iMod (inv_alloc N _ (bank_inv (γ1, γ2)) with "[Hown1 Hown2]") as "Hinv".
+    { iNext. iExists _, _; iFrame.
+      iPureIntro; auto. }
+    iModIntro.
+    iApply "HΦ".
+    iExists _, _, (γ1, γ2); iFrame.
+    iSplit; first eauto.
+    simpl.
+    iSplitL "Hlk1".
+    - iExists _; eautho with iFrame.
+    - iExists _; eautho with iFrame.
+Qed.
+
+
+End heap.
